\begin{align*}
  \lambda_2 &= \lambda_1 (1 - p_{e,1}) \\
  \lambda_3 &= \lambda_2 (1 - p_{e,2}) = \lambda_1 (1 - p_{e,1}) (1 - p_{e,2}) \\
  & \cdots \\
  \lambda_{r+1} &= \lambda_r (1-p_{e,r}) = \lambda_1 \prod_{k=1}^{r} (1 - p_{e,k})
  \text{, and, hence} \\
  \lambda_0 &= \lambda_1 \prod_{k=1}^{r+1} (1 - p_{e,k})
\end{align*}

The success rate, or end-to-end probability of successful receipt of packets at
the mobile station is hence

\begin{align*}
  p_{s,e2e} &= \prod_{k=1}^{r+1} (1 - p_{e,k})
\end{align*}

and the end-to-end error probability is then

\begin{align*}
  p_{e,e2e} &= 1 - p_{s,e2e} = 1 - \prod_{k=1}^{r+1} (1 - p_{e,k})
\end{align*}
